@prefix : <http://w3id.org/montolo/ns/montolo-voc#> .
@prefix cc: <http://creativecommons.org/ns#> .
@prefix qb: <http://purl.org/linked-data/cube#> .
@prefix dct: <http://purl.org/dc/terms/> .
@prefix owl: <http://www.w3.org/2002/07/owl#> .
@prefix rdf: <http://www.w3.org/1999/02/22-rdf-syntax-ns#> .
@prefix xml: <http://www.w3.org/XML/1998/namespace> .
@prefix xsd: <http://www.w3.org/2001/XMLSchema#> .
@prefix foaf: <http://xmlns.com/foaf/0.1/> .
@prefix frbr: <http://purl.org/vocab/frbr/core#> .
@prefix prov: <http://www.w3.org/ns/prov#> .
@prefix rdfs: <http://www.w3.org/2000/01/rdf-schema#> .
@prefix vann: <http://purl.org/vocab/vann/> .
@prefix voaf: <http://purl.org/vocommons/voaf#> .

<https://w3id.org/montolo/ns/montolo-voc#> rdf:type owl:Ontology ;
                                       vann:preferredNamespacePrefix "mov" ;
                                       vann:preferredNamespaceUri "https://w3id.org/montolo/ns/montolo-voc#" ;
                                       rdfs:label "MontoloVoc vocabulary"@en ;
                                       dct:title "MontoloVoc vocabulary"@en ;
                                       dct:description "The MontoloVoc vocabulary used to describe https://w3id.org/montolo"@en ;
                                       rdfs:comment """-Version 1.0.0: Rebranded from LOVCube vocabulary."""@en ;
                                       rdfs:comment """-Version 2.0.0: Fixed semantic issues and removed unused classes"""@en ;
                                       owl:versionIRI   <https://w3id.org/montolo/ns/montolo-voc/v2.0.0> ;
                                       owl:versionInfo "2.0.0" ;
                                       owl:priorVersion <https://w3id.org/montolo/ns/montolo-voc#> ;
                                       rdfs:seeAlso <https://w3id.org/montolo> ;
                                       dct:modified "2020-08-18"^^xsd:date ;
                                       dct:issued "2019-07-19"^^xsd:date ;
                                       dct:created "2019-07-19"^^xsd:date ;
                                       dct:rights "Copyright © Ghent University – imec – IDLab"@en ;
                                       cc:license <https://creativecommons.org/publicdomain/zero/1.0/> ;
                                       foaf:primaryTopic <https://w3id.org/montolo> ;
                                       dct:creator <https://sven-lieber.org/profile#me> ;
                                       dct:contributor <http://ben.de-meester.org/#me> ;
                                       dct:contributor :natadimou .

:natadimou rdf:type foaf:Person ;
  foaf:name "Anastasia Dimou"@en ;
  foaf:mbox "mailto:Anastasia.dimou@UGent.be" .

<https://sven-lieber.org/profile#me> rdf:type foaf:Person ;
                                     foaf:mbox "mailto:sven.lieber@ugent.be" ;
                                     foaf:name "Sven Lieber"@en .

<https://ben.de-meester.org/#me> rdf:type foaf:Person ;
                                 foaf:mbox "mailto:ben.demeester@ugent.be" ;
                                 foaf:name "Ben De Meester"@en .


#################################################################
#    Object Properties
#################################################################

:detectsRestrictionTypeExpression rdf:type owl:ObjectProperty ;
                                  rdfs:label "detects restriction type expression" ;
                                  rdfs:comment "Can be used to make the link between restriction types and restriction types expressions explicit." ;
                                  rdfs:domain :RestrictionTypeExpressionDetector ;
                                  rdfs:range :RestrictionTypeExpression .


:hasRestrictionTypeDefinition rdf:type owl:ObjectProperty ;
                              rdfs:label "has restriction type definition" ;
                              rdfs:comment "Links a restriction type to a specific version of a definition." ;
                              rdfs:domain :RestrictionType ;
                              rdfs:range :RestrictionTypeDefinitionVersion .


#################################################################
#    Classes
#################################################################

:Dataset 
  rdf:type owl:Class ;
  rdfs:label "Dataset" ;
  rdfs:comment "A dataset of ontology statistics which are both a datacube dataset (qb:DataSet) and a PROV-O entity (prov:Entity)." ;
  rdfs:subClassOf 
    qb:DataSet ,
    prov:Entity .


:RestrictionType
  rdf:type owl:Class ;
  rdfs:subClassOf
    frbr:Work ,
    prov:Entity ;
  rdfs:comment "A certain type of restriction, which can be an axiom or a constraint. One example is the restriction type 'disjoint classes'."@en ;
  rdfs:label "Restriction Type"@en .


:RestrictionTypeDefinition
  rdf:type owl:Class ;
  rdfs:subClassOf
    frbr:Work ,
    prov:Entity ;
  rdfs:label "Restriction Type Definition"@en ;
  rdfs:comment "A natural language definition of restriction types"@en .


:RestrictionTypeDefinitionVersion
  rdf:type owl:Class ;
  rdfs:label "Restriction Type Definition Version"@en ;
  rdfs:comment "A specific version of a definition for a restriction type."@en .


:RestrictionTypeExpression 
  rdf:type owl:Class ;
  rdfs:subClassOf
    frbr:Expression ,
    prov:Entity ;
  rdfs:comment "One possible expression of a restriction type. One example might be the expression 'owl:disjointWith' for the restriction type 'disjoint classes'."@en ;
  rdfs:label "Restriction Type Expression"@en .


:RestrictionTypeExpressionDetector
  rdf:type owl:Class ;
  rdfs:subClassOf 
    frbr:Work ,
    prov:Entity ;
  rdfs:comment "A piece of software which is able to detect a certain restriction type expression. Multiple versions of this detector might exist as separate entities"@en ;
  rdfs:label "Restriction Type Expression Detector"@en .


:RestrictionTypeExpressionDetectorVersion
  rdf:type owl:Class ;
  rdfs:subClassOf
    frbr:Expression ,
    prov:Entity ;
  rdfs:comment "A concrete version of a restriction type expression detector."@en ;
  rdfs:label "Restriction Type Expression Detector Version"@en .


:RestrictionTypeMeasure
  rdf:type owl:Class ;
  rdfs:subClassOf prov:Entity ;
  rdfs:label "Restriction Type Measure"@en ;
  rdfs:comment "A measure of a restriction type which follows the RDF Data Cube definition. Examples could be the 'occurrence' of a restriction type or 'hierarchy depth' etc."@en .


:RestrictionTypeStatistic
  rdf:type owl:Class ;
  rdfs:subClassOf
    qb:Observation ,
    prov:Entity ;
  rdfs:label "Restriction Type Statistic"@en ;
  rdfs:comment "A restriction type statistic basically is a RDF Data Cube observation about restriction type use, but also a PROV-O entity such that provenance of it can be expressed."@en .

:Repository
  rdf:type owl:Class ;
  rdfs:subClassOf prov:Entity ;
  rdfs:label "Repository"@en ;
  rdfs:comment "Any type of software repository from which input data is taken."@en .

:OntologyRepository 
  rdf:type owl:Class ;
  rdfs:subClassOf :Repository ;
  rdfs:label "Ontology Repository"@en ;
  rdfs:comment "A repository which hosts ontologies, examples could be Linked Open Vocabularies (LOV) or BioPortal."@en .

#################################################################
#    General axioms
#################################################################

[ rdf:type owl:AllDisjointClasses ;
   owl:members ( :RestrictionType
                 :RestrictionTypeDefinition
                 :RestrictionTypeExpression
                 :RestrictionTypeExpressionDetector
                 :RestrictionTypeExpressionDetectorVersion
                 :RestrictionTypeMeasure
                 :RestrictionTypeStatistic
               )
 ] .


